src/LibListSub.v
@@ -1,0 +1,322 @@
+(**************************************************************************
+* TLC: A library for Coq                                                  *
+* Sub-lists                                                               *
+**************************************************************************)
+
+Set Implicit Arguments.
+Generalizable Variables A B.
+Require Import Coq.Classes.Morphisms. (* for [Proper] instances *)
+Require Import LibTactics LibLogic LibReflect LibOperation
+ LibProd LibOption LibNat LibInt LibWf LibStruct LibRelation LibList.
+Local Open Scope nat_scope.
+Local Open Scope comp_scope.
+Global Close Scope list_scope.
+
+
+(* -------------------------------------------------------------------------- *)
+
+(* The [prefix] ordering on lists. *)
+
+Section Prefix.
+
+Variable A : Type.
+
+(* A definition in terms of concatenation. See also [LibListZ]. *)
+
+Definition prefix (ys xs : list A) :=
+  exists zs, ys ++ zs = xs.
+
+  (* TODO one could give an alternate definition of [prefix] as an
+     inductive predicate with two cases: [Nil/Cons] and [Cons/Cons].
+     This would give rise to a potentially useful induction principle.
+     Or just prove this induction principle directly. *)
+
+(* Ordering. *)
+
+Lemma prefix_reflexive:
+  forall xs,
+  prefix xs xs.
+Proof using.
+  intros. exists (@nil A). eapply app_nil_r.
+Qed.
+
+Lemma prefix_antisymmetric:
+  forall xs ys,
+  prefix xs ys ->
+  prefix ys xs ->
+  xs = ys.
+Proof using.
+  introv (ws&?) (zs&?). subst ys. rew_list in *.
+  forwards: app_eq_self_inv_l. { eauto. }
+  forwards: app_eq_nil_inv. { eauto. }
+  unpack. subst ws zs. rew_list. eauto.
+Qed.
+
+Lemma prefix_transitive:
+  forall xs ys zs,
+  prefix xs ys ->
+  prefix ys zs ->
+  prefix xs zs.
+Proof using.
+  introv [ xs' ? ] [ ys' ? ].
+  subst. rew_list. unfold prefix. eauto.
+Qed.
+
+(* [prefix] and [nil]. *)
+
+Lemma prefix_nil:
+  forall xs,
+  prefix nil xs.
+Proof using.
+  intros. exists xs. eapply app_nil_l.
+Qed.
+
+Lemma prefix_nil_inverse:
+  forall xs,
+  prefix xs nil ->
+  xs = nil.
+Proof using.
+  introv (ys&?).
+  forwards: app_eq_nil_inv. eauto.
+  unpack. eauto.
+Qed.
+
+(* [prefix] and [cons]. *)
+
+Lemma prefix_cons_inverse: (* TEMPORARY rename: [prefix_cons_r_inverse] *)
+  forall xs y ys,
+  prefix xs (y :: ys) ->
+  xs = nil \/ exists xs', xs = y :: xs' /\ prefix xs' ys.
+Proof using.
+  introv (zs&Heq).
+  destruct xs; [ eauto | right ].
+  rew_list in Heq. injects Heq.
+  unfold prefix. eauto.
+Qed.
+
+Lemma use_prefix_cons: (* TEMPORARY rename: [prefix_cons_l_inverse] *)
+  forall x xs ys,
+  prefix (x :: xs) ys ->
+  exists ys', ys = x :: ys'.
+Proof using.
+  introv [ slack ? ]. rew_list in *. exists (xs ++ slack). eauto.
+Qed.
+
+Lemma prefix_cons_cons:
+  forall x xs1 xs2,
+  prefix xs1 xs2 ->
+  prefix (x :: xs1) (x :: xs2).
+Proof using.
+  introv (ys&?). subst. exists ys. rew_list. eauto.
+Qed.
+
+Lemma prefix_cons_cons_inverse:
+  forall x1 x2 xs1 xs2,
+  prefix (x1 :: xs1) (x2 :: xs2) ->
+  x1 = x2 /\ prefix xs1 xs2.
+Proof using.
+  intros.
+  forwards: prefix_cons_inverse; eauto.
+  branches; unpack; try split; congruence.
+Qed.
+
+Lemma prefix_cons_cons_eq:
+  forall x xs1 xs2,
+  prefix (x :: xs1) (x :: xs2) = prefix xs1 xs2.
+Proof using.
+  intros. extens. split.
+  { eapply prefix_cons_cons_inverse. }
+  { eapply prefix_cons_cons. }
+Qed.
+
+(* [prefix] and [++]. *)
+
+Lemma prefix_concat:
+  forall xs ys zs,
+  prefix xs ys ->
+  prefix xs (ys ++ zs).
+Proof using.
+  unfold prefix. introv (ws&?). subst ys.
+  exists (ws ++ zs). rew_list. eauto.
+Qed.
+
+Lemma prefix_concat_simplify:
+  forall xs ys1 ys2,
+  prefix ys1 ys2 ->
+  prefix (xs ++ ys1) (xs ++ ys2).
+Proof using.
+  introv (ws&?). subst ys2. exists ws. rew_list. eauto.
+Qed.
+
+Lemma eliminate_common_prefix:
+  forall xs ys zs,
+  prefix (xs ++ ys) (xs ++ zs) ->
+  prefix ys zs.
+Proof using.
+  introv [ slack ? ]. exists slack.
+  rew_list in *.
+  eauto using app_cancel_l.
+Qed.
+
+Lemma prefix_app_r_inverse:
+  forall ys1 xs ys2,
+  prefix xs (ys1 ++ ys2) ->
+  prefix xs ys1 \/
+  exists ys2a, xs = ys1 ++ ys2a /\ prefix ys2a ys2.
+Proof using.
+  induction ys1 as [ | y ys1 ]; simpl; intros.
+  { right. exists xs. rew_list in *. eauto. }
+  { destruct xs as [ | x xs ].
+    { eauto using prefix_nil. }
+    { rew_list in *.
+      forwards: prefix_cons_cons_inverse. { eauto. } unpack. subst y.
+      forwards [ ? | (ys2a&?&?) ]: IHys1. { eauto. }
+      { eauto using prefix_cons_cons. }
+      { right. eexists ys2a. rew_list. subst xs. eauto. }
+    }
+  }
+Qed.
+
+(* [prefix] and [snoc]. *)
+
+Lemma prove_prefix_snoc:
+  forall x xs ys zs,
+  xs ++ x :: ys = zs ->
+  prefix (xs & x) zs.
+Proof using.
+  intros. exists ys. rew_list. eauto.
+Qed.
+
+Lemma use_prefix_snoc:
+  forall x xs ys zs,
+  prefix (xs & x) ys ->
+  ys = xs ++ zs ->
+  exists zs', zs = x :: zs'.
+Proof.
+  introv h ?. subst.
+  forwards: eliminate_common_prefix h.
+  eauto using use_prefix_cons.
+Qed.
+
+Lemma prefix_last: (* TEMPORARY should be: use_prefix_snoc *)
+  forall x xs ys,
+  prefix (xs & x) ys ->
+  prefix xs ys.
+Proof using.
+  introv [ zs ? ]. exists (x :: zs). rew_list in *. eauto.
+Qed.
+
+(* [prefix] and [length]. See also [LibListZ]. *)
+
+Lemma prefix_length:
+  forall ys xs,
+  prefix ys xs ->
+  length ys <= length xs.
+Proof using.
+  intros ys xs [ zs ? ]. subst xs. rew_list. math.
+Qed.
+
+Lemma prefix_snoc_length:
+  forall ys y xs,
+  prefix (ys & y) xs ->
+  length ys < length xs.
+Proof using.
+  intros ys y xs [ zs ? ]. subst xs. rew_list. math.
+Qed.
+
+(* [prefix] and [No_duplicates]. *)
+
+Lemma no_duplicates_prefix:
+  forall xs ys,
+  No_duplicates ys ->
+  prefix xs ys ->
+  No_duplicates xs.
+Proof using.
+  introv ? (zs&?). subst.
+  forwards: No_duplicates_inv_app; eauto.
+  tauto.
+Qed.
+
+End Prefix.
+
+Hint Resolve
+  prefix_reflexive
+  prefix_nil
+  prefix_cons_cons
+  prefix_concat
+  prefix_concat_simplify
+  prove_prefix_snoc
+: prefix.
+
+(* -------------------------------------------------------------------------- *)
+
+Section PrefixClosed.
+
+Variable A : Type.
+
+Implicit Types xs ys : list A.
+
+(* Prefix-closedness. *)
+
+Definition prefix_closed (P : list A -> Prop) :=
+  forall xs ys,
+  P ys ->
+  prefix xs ys ->
+  P xs.
+
+Lemma prefix_closed_nil:
+  forall (P : list A -> Prop) xs,
+  prefix_closed P ->
+  P xs ->
+  P nil.
+Proof using.
+  eauto with prefix.
+Qed.
+
+(* Prefix closure. *)
+
+Definition prefix_closure (P : list A -> Prop) : list A -> Prop :=
+  fun xs => exists ys, prefix xs ys /\ P ys.
+
+Definition prefix_closure_alt (P : list A -> Prop) : list A -> Prop :=
+  fun xs => exists ys, P (xs ++ ys).
+
+Lemma prefix_closure_eq:
+  forall P,
+  prefix_closure P = prefix_closure_alt P.
+Proof using.
+  intros. extens; intros xs; split; unfold prefix_closure, prefix_closure_alt, prefix.
+  { introv (ys&(zs&?)&?). subst. eauto. }
+  { introv (ys&?). eauto. }
+Qed.
+
+Lemma prefix_closure_is_prefix_closed:
+  forall P,
+  prefix_closed (prefix_closure P).
+Proof.
+  unfold prefix_closed, prefix_closure.
+  introv (zs&?&?). eauto using prefix_transitive.
+Qed.
+
+(* The relation [fun xs => prefix xs ys] is the prefix closure of the
+   singleton [ys]. Thus, it is prefix-closed. *)
+
+Lemma prefix_closure_singleton:
+  forall ys : list A,
+  (fun xs => prefix xs ys) = prefix_closure (= ys).
+Proof using.
+  intros. extens; intros xs. unfold prefix_closure.
+  split. eauto. intros (?&?&?). subst. eauto.
+Qed.
+
+Lemma prefix_closed_prefix:
+  forall ys : list A,
+  prefix_closed (fun xs => prefix xs ys).
+Proof using.
+  intros. rewrite prefix_closure_singleton.
+  eapply prefix_closure_is_prefix_closed.
+Qed.
+
+End PrefixClosed.
+
+
